update

theories/Evens.v
@@ -7,3 +7,226 @@ From Coq Require Import Init.Nat.
 From Coq Require Import Lia.
 
 Import ListNotations.
+
+
+
+Fixpoint selectEvens (l : list nat): list nat :=
+  match l with
+  | [] => []
+  | (h :: t) => 
+    if even h
+    then h :: selectEvens t
+    else selectEvens t
+  end.
+  
+Check selectEvens [1;2;3;4;100;101;300;299] = [2;4;100;300].
+
+Inductive selectEvensInd : list nat -> list nat -> Prop :=
+  | SelectEvensEmpty : selectEvensInd [] []
+  | SelectEvensEven :
+      forall x l selected,
+      selectEvensInd l selected ->
+      even x = true ->
+      selectEvensInd (x :: l) (x :: selected)
+  | SelectEvensOdd :
+      forall x l selected,
+      selectEvensInd l selected ->
+      even x = false ->
+      selectEvensInd (x :: l) selected
+  .
+
+Example selectEvensInd_example_1 : selectEvensInd [1;2;3;4;100;101;300;299] [2;4;100;300].
+Proof. repeat constructor. Qed.
+Example selectEvensInd_example_2 : selectEvensInd [1] [1] -> False.
+Proof. intros H. inversion H; subst. discriminate. inversion H2. Qed.
+
+  
+Theorem selectEvensInd_preserves_in :
+  forall l selected a, selectEvensInd l selected -> In a selected -> In a l.
+Proof.
+  intros l selected a Hsel. generalize dependent a.
+  induction Hsel; subst.
+  - auto.
+  - intros a Hin. destruct Hin.
+    + subst. now left.
+    + specialize (IHHsel _ H0).
+      now right.
+  - intros a Hin. specialize (IHHsel _ Hin).
+    now right.
+  Qed.
+
+Theorem selectEvensInd_same_as_selectEvens :
+  forall l selected, selectEvensInd l selected -> selectEvens l = selected.
+Proof.
+  intros l selected H.
+  induction H.
+  - auto.
+  - simpl.
+    now rewrite H0,IHselectEvensInd.
+  - simpl.
+    now rewrite H0,IHselectEvensInd.
+  Qed.
+
+Theorem selectEvens_same_as_selectEvensInd :
+  forall l selected, selectEvens l = selected -> selectEvensInd l selected.
+Proof.
+  (*
+  intros l selected. generalize dependent l.
+  induction selected.
+  - destruct l.
+    + intros. constructor.
+    + simpl.
+  *)
+  induction l.
+  - simpl. intros selected H. rewrite <- H. constructor.
+  - simpl. intros selected H.
+    destruct (even a) eqn:E.
+    + destruct selected; try discriminate.
+      inversion H; subst.
+      constructor; try assumption.
+      now apply IHl.
+    + constructor; try assumption.
+      now apply IHl.
+  Qed.
+
+Theorem selectEvensPreservesIn : forall l a, In a (selectEvens l) -> In a l.
+Proof.
+  (*
+  intros l.
+  remember (selectEvens l) as c.
+  symmetry in Heqc.
+  apply selectEvens_same_as_selectEvensInd in Heqc.
+  intros a H. apply selectEvensInd_preserves_in with c; assumption. *)
+  intros l a HInaselect.
+  remember (selectEvens l) as c eqn:Heqc. symmetry in Heqc.
+  (** Turn [selectEvens l = c] into [selectEvensInd l c]. *)
+  apply selectEvens_same_as_selectEvensInd in Heqc.
+  (** Induction over [selectEvensInd l c] *)
+  induction Heqc.
+  - (** Constructor [SelectEvensEmpty : selectEvensInd [] []].
+        This is the case where [In a []], which we know can't happen. *)
+    auto.
+  - (** Constructor [SelectEvensEven : selectEvensInd l selected -> even x = true -> selectEvensInd (x :: l) (x :: selected)].
+        This is the case where we know [In a (x :: selected)]. *)
+     destruct HInaselect.
+    + (** Here we know [x = a] and we need to prove [In a (x :: l)]. *)
+      subst. now left.
+    + (** Here we know [In a selected] and we need to prove [In a (x :: l)].
+          We use the induction hypothesis: [In a selected -> In a l]. *)
+      right. apply IHHeqc. assumption.
+  - (** Constructor [SelectEvensOdd : selectEvensInd l selected -> even x = false -> selectEvensInd (x :: l) selected].
+        Similar to the previous case. *)
+    right. apply IHHeqc. assumption.
+  Qed.
+  
+Theorem selectEvensPreservesIn2 : forall l a, In a (selectEvens l) -> In a l.
+Proof.
+  (*
+  intros l.
+  remember (selectEvens l) as c eqn:Heqc. symmetry in Heqc.
+  induction l.
+  - intros l HInaselect. simpl in Heqc. subst. destruct HInaselect.
+  - simpl in Heqc.
+    intros x HInaselect.
+    destruct (even a) eqn:E.
+    * rewrite <- Heqc in HInaselect.
+      destruct HInaselect.
+      + subst. now left.
+      + right.
+  *)
+  induction l.
+  - simpl. auto.
+  - simpl.
+    intros b H.
+    destruct (even a) eqn:E.
+    + destruct H.
+      * subst. now left.
+      * right. apply IHl. apply H.
+    + right. apply IHl. auto.
+  Qed.
+  
+(*
+Theorem selectEvensIndPreservesSorted :
+  forall l selected, selectEvensInd l selected -> LocallySorted le l -> LocallySorted le selected.
+Proof.
+  (*
+  intros l selected H.
+  induction H.
+  - auto.
+  - intros Hsorted.
+    inversion Hsorted; subst.
+    * Print LocallySorted.
+    constructor.
+    * apply IHselectEvensInd. auto.
+    * 
+    apply IHselectEvensInd in H3.
+    constructor.
+  *)
+  (*
+  intros l selected H Hsorted. generalize dependent H. generalize dependent selected.
+  induction Hsorted; intros selected Hselect.
+  - inversion Hselect. constructor.
+  - inversion Hselect; subst.
+    + inversion H1; subst. constructor.
+    + inversion H1; subst. constructor.
+  - inversion Hselect; subst.
+    + inversion H2; subst.
+      * constructor.
+        -- apply IHHsorted. apply H2.
+        -- assumption.
+      * specialize (IHHsorted _ H2).
+        inversion IHHsorted; subst.
+        -- constructor.
+        --  
+  *)
+  (*
+  intros l. induction l.
+  - intros ? Hsel ?. inversion Hsel; subst. constructor.
+  - intros selected Hsel Hsor.
+    inversion Hsor; subst.
+    + apply IHl.
+      * 
+  *)
+  intros l selected. generalize dependent l.
+  induction selected.
+  - intros l Hsel Hsor. constructor.
+  - intros l Hsel  Hsor.
+    inversion Hsel; subst.
+    + inversion Hsor; subst.
+      * inversion H2; subst. constructor.
+      * specialize (IHselected _ H2 H1).
+        inversion H2; subst.
+        -- constructor; try assumption.
+        -- *)
+
+
+Theorem selectEvensInd_preserves_forall :
+  forall f l select, selectEvensInd l select -> Forall f l -> Forall f select.
+Proof.
+  intros f l select Hsel.
+  induction Hsel; intros Hfor.
+  - assumption.
+  - inversion Hfor; subst.
+    constructor; try auto.
+  - inversion Hfor; subst. auto.
+  Qed.  
+
+Theorem selectEvensIndPreservesSorted :
+  forall l selected, selectEvensInd l selected -> StronglySorted le l -> StronglySorted le selected.
+Proof.
+  (*
+  intros l. induction l; simpl; intros selected Hsel Hsor.
+  - inversion Hsel; subst. constructor.
+  - inversion Hsel; subst; inversion Hsor; subst.
+    + specialize (IHl _ H1 H2).
+      constructor; try assumption.
+  *)
+  intros l selected Hsel Hsor. generalize dependent Hsel. generalize dependent selected.
+  induction Hsor; intros selected Hsel.
+  - inversion Hsel; subst. constructor.
+  - inversion Hsel; subst.
+    + constructor.
+      * apply IHHsor. assumption.
+      * apply selectEvensInd_preserves_forall with l; auto.
+    + now apply IHHsor.
+  Qed.
